20250603

src/Automaton.v
@@ -20,7 +20,7 @@ Declare Scope language_scope.
 Delimit Scope automaton_scope with LANG.
 
 Structure automaton{state symbol:finType} :=
-    {delta:symbol -> (Rel state state); init:Rel i state; final:Rel i state}.
+    {delta:symbol -> (Rel state state); init:Rel i state; final:Rel state i}.
 
 Fixpoint dstar{state symbol:finType}(d:symbol -> (Rel state state))(w:seq symbol):(Rel state state):=
 match w with
@@ -28,272 +28,1083 @@ match w with
 |s::w' => (d s) ・ (dstar d w')
 end.
 Definition accept{state symbol:finType}(M:@automaton state symbol)(w:seq symbol):Prop :=
-(init M) ・ (dstar(delta M)w) ・ (final M)# = Id i.
+(init M) ・ (dstar(delta M)w) ・ (final M) = Id i.
+Notation " 'L' M " := (accept M) (at level 50, left associativity, 
+                                      only parsing):automaton_scope.
+
+Open Scope language_scope.
+Definition language {symbol:finType}:=seq symbol->Prop.
+Definition rev_l {symbol:finType}(l:language):language:=
+fun s:seq symbol=>l (rev s).
+Notation "l '^r'" := (rev_l l) (at level 30):language_scope.
+Definition preimage_l {symbol:finType}(a:symbol)(l:language):language:=
+fun w:seq symbol=> l (a::w).
+Definition preimage_r {symbol:finType}(a:symbol)(l:language):language:=
+fun w:seq symbol=> l (rcons w a).
+
+Lemma preimage_assoc {symbol:finType}:forall(a b:symbol)(l:language),
+preimage_r b (preimage_l a l) = preimage_l a (preimage_r b l).
+Proof.
+move=>a b l.
+by rewrite/preimage_l/preimage_r.
+Qed.
+
+Definition preimage_lang_l {symbol:finType}(l l':language):language:=
+fun v:seq symbol=>exists u, l u /\ l' (u++v).
+Definition preimage_lang_r {symbol:finType}(l l':language):language:=
+fun v:seq symbol=>exists u, l u /\ l' (v++u).
+
+Lemma preimage_lang_assoc {symbol:finType}:forall(A B l:language),
+forall w:seq symbol, preimage_lang_r B (preimage_lang_l A l) w <-> preimage_lang_l A (preimage_lang_r B l) w.
+Proof.
+move=>A B l w.
+rewrite/preimage_lang_l/preimage_lang_r.
+split=>[][]u[]H[]v[]H0 H1;exists v;(split;[done|]);exists u;(split;[done|]);
+by rewrite catA in H1 *.
+Qed.
+
+Definition cup_lang{symbol:finType}(x y:language):language:=
+fun s:seq symbol=>x s\/y s.
+Notation "x '∪' y" := (cup_lang x y)(at level 50):language_scope.
+Definition cap_lang{symbol:finType}(x y:language):language:=
+fun s:seq symbol=>x s/\y s.
+Notation "x '∩' y" := (cap_lang x y) (at level 50):language_scope.
+Definition prod_lang{symbol:finType}(x y:language):language:=
+fun s:seq symbol=>exists a b,s=a++b/\x a/\y b.
+Notation "x '・' y" := (prod_lang x y) (at level 50):language_scope.
+Definition phi{symbol:finType}:@language symbol := fun x=>False.
+Definition eps{symbol:finType}:language := fun s:seq symbol=>s = nil.
+Definition singl{symbol:finType}(s:symbol):language := fun x=> x = [::s].
+Fixpoint power_l {symbol : finType}(n : nat)(l : @language symbol): language :=
+  match n with
+  | 0 => eps
+  | S n' => l ・ power_l n' l 
+  end.
+Notation "l '^' n" := (power_l l n) (at level 30):language_scope.
+Definition times_l{symbol:finType}(l:language):language:=
+fun s:seq symbol=> exists n,power_l n l s.
+Notation "l '^*'" := (times_l l) (at level 30):language_scope.
+Definition plus_l{symbol:finType}(l:language):language:=
+fun s:seq symbol=> exists n,power_l(S n)l s.
+Notation "l '^+'" := (plus_l l) (at level 30):language_scope.
+Definition comp_lang{symbol:finType}(l:language):language:=
+fun s:seq symbol=>~ l s.
+Notation "l '^c'" := (comp_lang l) (at level 30):language_scope.
 
 Definition deterministic {state symbol:finType}(M:@automaton state symbol):Prop:=
 (forall s:symbol,function_r(delta M s))/\function_r(init M).
 
-Definition plusM{state1 state2 symbol:finType}(M:@automaton state1 symbol)(M':@automaton state2 symbol):automaton :=
-    {|delta := fun x=>(@inl_r state1 state2)#・((delta M)x)・(@inl_r state1 state2)∪((@inr_r state1 state2) #・((delta M')x)・(@inr_r state1 state2)); init:=(init M)・(@inl_r state1 state2)∪((init M')・(@inr_r state1 state2)); final := (final M)・(@inl_r state1 state2)∪((final M')・(@inr_r state1 state2))|}.
-Notation "M '+' M'" := (plusM M M') (at level 50, left associativity, 
-                                      only parsing):automaton_scope.
+Definition is_regular {symbol:finType}(l:language):Prop:=
+exists (state:finType)(M:@automaton state symbol),forall w,l w <-> accept M w. 
+Close Scope language_scope.
+
+Definition plusM {state state' symbol:finType}(M:@automaton state symbol)(M':@automaton state' symbol):automaton :=
+    {|delta := fun x=>Rel_sum(delta M x・@inl_r _ state')(delta M' x・@inr_r state _);
+      init  := Rel_sum(init M #)(init M' #)#;
+      final := Rel_sum(final M)(final M')|}.
+Notation "M '+' M'" := (plusM M M') (at level 50, left associativity):automaton_scope.
+Definition timesM {state state' symbol:finType}(M:@automaton state symbol)(M':@automaton state' symbol):automaton :=
+    {|delta := fun s=>Rel_prod(fst_r state state'・delta M s)(snd_r state state'・delta M' s);
+      init := Rel_prod(init M)(init M');
+      final := Rel_prod(final M #)(final M' #)# |}.
+Notation "M '×' M'" := (timesM M M') (at level 50, left associativity):automaton_scope.
+Definition revM {state symbol:finType}(M:@automaton state symbol):=
+    {|delta := fun x=>delta M x #; init  := final M #; final := init M # |}.
+Definition concatM {state state' symbol:finType}(M:@automaton state symbol)(M':@automaton state' symbol):automaton:=
+    {|delta := fun x =>( @inl_r _ state' #・delta M x・@inl_r _ state')∪(Rel_sum(final M・init M')(Id _)・delta M' x・@inr_r state _);
+      init  := init M・(Rel_sum(Id _)(init M' #・final M #)#);
+      final := (Rel_sum(final M・init M')(Id _))・final M'|}.
+Definition phiM{symbol:finType}:@automaton _ symbol:= {|delta := fun x=>φ i i; init  := φ i i;final := φ i i|}.
+Definition epsM{symbol:finType}:@automaton _ symbol:={|delta := fun x=>φ i i;init:=Id i;final:=Id i|}.
+Definition singlM{symbol:finType}(s:symbol):automaton :=
+    {|delta := fun (x:symbol)(a b:bool)=>a/\x=s/\not b;
+      init  := fun (x:i)(a:bool)=>is_true a;
+      final := fun (a:bool)(x:i)=>not (is_true a)|}.
+Definition compM{state symbol:finType}(M:@automaton state symbol):automaton:=
+    {|delta := delta M; init := init M; final := final M ^|}.
+Definition plus_nfa {state symbol:finType}(M:@automaton state symbol):automaton :=
+    {|delta := fun x=>(delta M x∪(delta M x・(final M・init M)));
+      init  := init M;
+      final := final M|}.
 
 
-Fixpoint delta_convert'{state:finType}(s:seq state)(R:Rel state state):state->Prop:=
-match s with
-|nil => fun x:state=>False
-|h::s' => fun x:state=>R h x\/delta_convert' s' R x
-end.
-Definition delta_convert{state:finType}(s:{set state})(R:Rel state state):{set state}:=
-[set x|is_true_inv((delta_convert'[seq x <- enum state | x \in s]R)x)].
+Lemma is_true_false:forall P, ~P <-> is_true_inv P = false.
+Proof.
+split=>H.
+rewrite/is_true_inv.
+move : (IndefiniteDescription.constructive_indefinite_description (fun b : bool => P <-> is_true b) (is_true_inv0 P)) =>[][]H0.
+by rewrite H0 in H.
+done.
+case:(Classical_Prop.classic P);[move=>/is_true_id H0|done].
+by rewrite H0 in H.
+Qed.
 
-Theorem NFA_DFA_equiv{symbol:finType}(w:seq symbol):
-(exists (state:finType)(M:@automaton state symbol),accept M w) <-> (exists (state:finType)(M':@automaton state symbol),deterministic M'/\accept M' w).
-split;move=>[state][M];[move=>H|by move=>[_ H];exists state,M].
-exists (finset_set_of__canonical__fintype_Finite state).
+Theorem NFA_DFA_equiv {state symbol:finType}(M:@automaton state symbol):
+exists(state':finType)(M':@automaton state' _),deterministic M'/\
+(forall w,accept M w <-> accept M' w).
+
 destruct M.
-exists {|delta:= fun (s:symbol)(x y:{set state})=>delta_convert x(delta0 s) = y;
+exists _,{|delta:= fun (s:symbol)(x y:{set state})=>[set z | is_true_inv(exists2 w, w \in x & delta0 s w z)] = y;
          init:= fun (x:i)(y:{set state})=>[set x|is_true_inv(init0 tt x)]=y;
-         final:= fun(x:i)(y:{set state})=>y:&:[set x|is_true_inv(final0 tt x)]<>set0|}.
+         final:= fun(y:{set state})(x:i)=>y:&:[set x|is_true_inv(final0 x tt)]<>set0|}.
+
 split.
-rewrite/deterministic.
+rewrite/deterministic/=.
 split.
 move=>s.
 rewrite/=/function_r/total_r/univalent_r.
 split.
 move=>x y{}H.
 have{}H:y=x;[done|subst].
-by exists (delta_convert x(delta0 s)).
-case=>alpha x.
-case=>y{}H.
-admit. 
-
-
-
-
-Theorem plusP{state1 state2 symbol:finType}(M:@automaton state1 symbol)(M':@automaton state2 symbol)(w:seq symbol):
-accept M w\/accept M' w <-> accept (M+M')%AUTO w.
-Proof.
-rewrite/accept.
+by exists [set z | is_true_inv (exists2 w0 : state, w0  \in x & delta0 s w0 z)].
+case=>alpha x[]y[]{}H H1.
+rewrite/inverse in H.
+by subst.
+rewrite/=/function_r/total_r/univalent_r.
 split.
-case=>H;
-(have:Id i tt tt;[done|]);
-rewrite-{1}H;
-case=>b[]{H};
-case=>a[]H H1 H2;
-apply/inc_antisym_eq;
-(split;[by rewrite unit_identity_is_universal|]=>x y);
-destruct x,y=>_;
-[move:(@inl_id state1 state2)|move:(@inr_id state1 state2)];
-move/inc_antisym_eq=>[_ H3];
-[have H4:Id state1 a a;[done|]|have H4:Id state2 a a;[done|]];
-move:(H3 a a H4)=>{}H4;
-case:H4=>a'[H4 H5];
-[have H6:Id state1 b b;[done|]|have H6:Id state2 b b;[done|]];
-move:(H3 b b H6)=>{}H6;
-case:H6=>b'[H6 H7];
-exists b';
-(split;[exists a';split|]).
-rewrite/=/cup/cupP.
-exists (init M ・ inl_r state1 state2).
-by split;[left|exists a].
-move:a a'{H}H1 H4 H5.
-elim:w.
-simpl=>a a' H.
-have{}H:a=b;[done|].
-subst=>H1{}H2.
-rewrite-inl_inr_cup_id/cup/cupP.
-exists(inl_r state1 state2 # ・ inl_r state1 state2).
-by split;[left|exists b].
-move=>h w H a a'.
-simpl.
-case=>c[H1{}H2 H4 H5].
-have H8:Id state1 c c;[done|].
-move:(H3 c c H8)=>{}H8.
-case:H8=>c'[H8 H9].
-move:(H c c' H2 H8 H9)=>{}H.
-exists c'.
-split.
-rewrite/cup/cupP.
-exists((inl_r state1 state2 # ・ delta M h) ・ inl_r state1 state2).
-by split;[left|exists c;split;[exists a|]].
-done.
-rewrite/=/cup/cupP/inverse.
-exists(final M ・ inl_r state1 state2).
-by split;[left|exists b].
-rewrite/=/cup/cupP.
-exists (init M' ・ inr_r state1 state2).
-by split;[right|exists a].
-move:a a'{H}H1 H4 H5.
-elim:w.
-simpl=>a a' H.
-have{}H:a=b;[done|].
-subst=>H1{}H2.
-rewrite-inl_inr_cup_id/cup/cupP.
-exists(inr_r state1 state2 # ・ inr_r state1 state2).
-by split;[right|exists b].
-move=>h w H a a'.
-simpl.
-case=>c[H1{}H2 H4 H5].
-have H8:Id state2 c c;[done|].
-move:(H3 c c H8)=>{}H8.
-case:H8=>c'[H8 H9].
-move:(H c c' H2 H8 H9)=>{}H.
-exists c'.
-split.
-rewrite/cup/cupP.
-exists((inr_r state1 state2 # ・ delta M' h) ・ inr_r state1 state2).
-by split;[right|exists c;split;[exists a|]].
-done.
-rewrite/=/cup/cupP/inverse.
-exists(final M' ・ inr_r state1 state2).
-by split;[right|exists b].
+move=>x y _.
+destruct x,y.
+rewrite/composite.
+by exists [set x | is_true_inv (init0 tt x)].
+case=>alpha x[]y[]{}H H1.
+rewrite/inverse in H.
+by subst.
 
-move=>H;have :Id i tt tt;[done|];rewrite-{1}H.
-case=>b'[].
-case=>a'[].
-case=>alpha[][]{}H;subst=>H H1.
-case=>gamma[][]H2;subst=>H2.
-left.
-case:H=>a[H H3].
-case:H2=>b[H2 H4].
-apply/inc_antisym_eq;
-(split;[by rewrite unit_identity_is_universal|]=>x y);
-destruct x,y=>_.
-exists b.
+move=>w.
+rewrite/accept/=.
 split.
-exists a.
-split.
-done.
-move:a' a H3 H1{H}.
-elim:w.
-simpl=>a' a H H1.
-have{}H1:a'=b'.
-done.
-subst.
-rewrite-(@inl_id _ state2).
-by exists b'.
-move=>h w H a' a H1.
-simpl.
-case=>c'[].
-rewrite/cup/cupP.
-case=>alpha[][]H3;subst.
-case=>c[].
-case=>d[]H3.
-have:(inl_r state1 state2 ・ inl_r state1 state2 #) a d.
-by exists a'.
-rewrite inl_id=>H5.
-have{}H5:a=d.
-done.
-subst=>H5 H6 H7.
-move:(H c' c H6 H7)=>{}H.
-by exists c.
-case=>x[].
-case=>y[]H5.
-have:(inl_r state1 state2・inr_r state1 state2 #) a y.
-by exists a'.
-by rewrite inl_inr_empty.
-done.
-
-case:H=>a[]H H3.
-case:H2=>b[]H2 H4.
-exfalso.
-move:a' a{H}H3 H1.
-elim:w.
-move=>a' a H1 H3.
-have{}H5:a'=b'.
-done.
-subst.
-have:(inl_r state1 state2・inr_r state1 state2 #) a b.
-by exists b'.
-by rewrite inl_inr_empty.
-move=>h w H1 a' a H3.
-simpl.
-case=>c'[].
-case=>alpha[][]H5;subst.
-case=>c[]H5 H6 H7.
-by move:(H1 c' c H6 H7).
-case=>x[].
-case=>y[]H5.
-have:(inl_r state1 state2 ・ inr_r state1 state2 #) a y.
-by exists a'.
-by rewrite inl_inr_empty.
-case:H=>a[H H2].
-case=>alpha[][]H3;subst.
-case=>b[]H3 H4.
-exfalso.
-move:w b' b{H3}H4 H1.
-have{}H:(forall (b' : Datatypes_sum__canonical__fintype_Finite state1 state2)
-(b : state1), inl_r state1 state2 b b' ->
-dstar (delta (plusM M M')) nil a' b' -> False).
-move=>b' b{}H H1.
-have H3:a'=b'.
-done.
-subst.
-have:(inr_r state1 state2・inl_r state1 state2 #) a b.
-by exists b'.
-by rewrite inr_inl_empty.
-apply/(last_ind H)=>w t{}H b' b H1.
-have H3:forall (d:symbol->Rel(Datatypes_sum__canonical__fintype_Finite state1 state2)(Datatypes_sum__canonical__fintype_Finite state1 state2))
-(l:seq symbol)(t:symbol), dstar d(rcons l t) = (dstar d l)・(d t).
-move=>d.
-elim.
-move=>t0.
-by rewrite/= comp_id_l comp_id_r.
-move=>h l H3 t0.
-by rewrite/=H3 comp_assoc.
-rewrite{}H3.
-case=>c'[]H3.
-case=>alpha[][]H4;subst.
-case=>c[]H4 H5.
-have:(inl_r state1 state2・inl_r state1 state2 #)b c.
-by exists b'.
-rewrite inl_id=>H6.
-have{}H6:c=b.
-done.
-subst.
-case:H4=>c[]H6.
-by move:(H c' c H6 H3).
-case=>x[_] {}H.
-have:(inl_r state1 state2・inr_r state1 state2 #)b x.
-by exists b'.
-by rewrite inl_inr_empty.
-case=>b[H3 H4].
-right.
-apply/inc_antisym_eq;
-(split;[by rewrite unit_identity_is_universal|]=>x y);
-destruct x,y=>_.
-exists b.
-split;[|done].
-exists a.
+have H:Id i tt tt;[done|move=>H1;rewrite-{}H1 in H].
+Rel_simpl;[by rewrite unit_identity_is_universal|move=>[][] _].
+case:H=>b[][]a[]H H1 H2.
+rewrite comp_assoc.
+exists [set x | is_true_inv (init0 tt x)].
 split;[done|].
-move:a' a H2 H1{H H3}.
+move:init0 a H H1.
 elim:w.
-simpl=>a' a H H1.
-have{}H1:b'=a'.
+move=>init0 a H H1.
+have{}H1:b=a;[done|subst].
+exists [set x | is_true_inv (init0 tt x)].
+split;[done|].
+rewrite/not=>H1.
+have:a\in set0.
+rewrite-H1!in_set(_:is_true_inv (init0 tt a));by apply/is_true_id.
+by rewrite in_set0.
+move=>h w H init0 a H1.
+simpl=>[][]c[]H3 H4.
+have H5:(init0・delta0 h)tt c.
+by exists a.
+rewrite comp_assoc.
+exists [set z | is_true_inv
+(exists2 w0 : state,
+w0  \in [set x | is_true_inv (init0 tt x)] & delta0 h w0 z)].
+split;[done|].
+move:(H (init0 ・ delta0 h)c H5 H4).
+rewrite(_:[set z | is_true_inv
+(exists2 w0 : state,
+w0  \in [set x | is_true_inv (init0 tt x)] & delta0 h w0 z)]=[set x | is_true_inv ((init0 ・ delta0 h) tt x)]).
 done.
-subst.
-rewrite-(@inr_id state1).
+rewrite/composite.
+apply/setP=>x.
+rewrite!in_set.
+have H6:forall P Q:Prop,(P<->Q) -> (is_true_inv P=is_true_inv Q).
+move=>P Q{}H.
+case_eq(is_true_inv P)=>{}H1;case_eq(is_true_inv Q)=>{}H2;[done| | |done].
+by have:is_true_inv Q;[by apply/is_true_id/H/is_true_id|rewrite H2].
+by have:is_true_inv P;[by apply/is_true_id/H/is_true_id|rewrite H1].
+apply/H6.
+split=>[][]y.
+rewrite in_set=>/is_true_id{}H{}H1.
+by exists y.
+move=>[]{}H{}H1.
+by exists y;[rewrite in_set;apply/is_true_id|].
+
+move=>H.
+have:Id i tt tt;[done|rewrite-{1}H].
+move=>[]b[][]a[]{}H H0 H1.
+Rel_simpl;[by rewrite unit_identity_is_universal|move=>[][] _].
+have:exists b',b'\in b /\ final0 b' tt.
+move:(H1)=>/eqP/set0Pn[]b'.
+rewrite in_setI in_set=>/andP[]H2 H3.
+exists b'.
+by split;[|apply/is_true_id].
+case=>b'[]H2 H3.
+exists b'.
+split;[|done].
+have set0dstar:forall w,dstar (fun (s : symbol) (x : {set state}) =>
+[eta eq [set z | is_true_inv (exists2 w : state, w  \in x & delta0 s
+w z)]]) w set0 b -> False.
+move{H0}=>{}w.
+elim:w=>[|h w{}H].
+rewrite/==>{}H.
+have{}H:b=set0;[done|subst;by rewrite in_set0 in H2].
+
+rewrite/==>[][]{}a[]H0.
+have{}H0:a=set0.
+rewrite-{}H0.
+apply/setP=>x.
+rewrite in_set in_set0.
+apply/is_true_false=>[][]x0.
+by rewrite in_set0.
+by rewrite H0.
+
+case_eq(a == set0)=>/eqP H4.
+rewrite H4 in H0.
+by move:(set0dstar _ H0).
+
+move:{final0 H1 H3}init0 a H4 H H0.
+elim:w=>[|h w H0]init0 a H4 H.
+rewrite/==>H0.
+have{}H0:b = a;[done|subst].
+exists b'.
+rewrite in_set in H2 *.
+by move:(H2)=>/is_true_id.
+
+rewrite/==>[][]c[]H1 H3.
+move:(H0(init0・delta0 h)c)=>{}H0.
+case_eq(c==set0)=>/eqP H5.
+rewrite H5 in H3.
+by move:(set0dstar _ H3).
+move:(H5)=>/H0{}H0.
+have H6:[set x | is_true_inv ((init0 ・ delta0 h) tt x)] = c.
+rewrite-H1.
+apply/setP=>x.
+rewrite!in_set.
+have{}H:(init0 ・ delta0 h) tt x <->exists2 w0 : state, w0  \in a & delta0 h w0 x.
+split.
+case=>a'[]{}H0{}H1.
+exists a'.
+rewrite-H in_set.
+by apply/is_true_id.
+done.
+case=>a'.
+rewrite-H in_set=>/is_true_id{}H{}H1.
 by exists a'.
-move=>h w H a' a H1.
-simpl.
-case=>c'[].
-case=>alpha[][]H2;subst.
-case=>c[].
-case=>d[]H2.
-have:(inr_r state1 state2・inl_r state1 state2 #)a d.
-by exists a'.
-by rewrite inr_inl_empty.
-case=>c[].
-case=>d[]H2.
-have{}H2:(inr_r state1 state2・inr_r state1 state2 #)a d.
-by exists a'.
-have{}H2:d=a.
-by rewrite inr_id in H2.
-subst=>{}H1 H2 H3.
-move:(H c' c H2 H3)=>{}H.
-by exists c.
+case_eq(is_true_inv ((init0 ・ delta0 h) tt x)).
+move=>/is_true_id/H{}H0.
+symmetry.
+by apply/is_true_id.
+rewrite-is_true_false=>{}H0.
+symmetry.
+apply/is_true_false/H/H0.
+
+move:(H0 H6 H3)=>[]c'[][]a'[]{}H{}H0{}H1.
+exists a'.
+split.
+done.
+by exists c'.
+Qed.
+
+Open Scope language_scope.
+Open Scope automaton_scope.
+Theorem regular_cup {symbol:finType}(l l':@language symbol):
+is_regular l/\is_regular l'->is_regular (l∪l').
+Proof.
+Close Scope language_scope.
+rewrite/is_regular=>[][][]state[]M H[]state'[]M' H'.
+exists (sum state state').
+exists (M + M') => w.
+rewrite/cup_lang{}H{}H'/accept.
+
+suff H:(init (plusM M M') ・ dstar (delta (plusM M M')) w) ・ final (plusM M M') = 
+((init M ・ dstar (delta M) w) ・ final M )∪((init M' ・ dstar (delta M') w) ・ final M').
+rewrite{}H.
+split=>[|H].
+case=>H;[rewrite cup_comm|];
+by rewrite H unit_identity_is_universal cup_universal.
+rewrite-{}H.
+case:( @unit_empty_or_universal((init M ・ dstar (delta M) w) ・ final M))=>H;
+rewrite H cup_comm;[rewrite cup_empty|rewrite cup_universal];by[right|left].
+
+destruct M,M';simpl.
+move:init0 init1.
+elim:w=>[|h w H]init0 init1.
+by rewrite/=!comp_id_r sum_comp inv_invol inv_invol.
+move:(H(init0・delta0 h)(init1・delta1 h))=>{}H.
+rewrite/=-!comp_assoc-{}H.
+f_equal.
+by rewrite sum_comp/Rel_sum inv_cup_distr!comp_inv!inv_invol!comp_assoc.
 Qed.
 
 
+Open Scope language_scope.
+Theorem regular_cap {symbol:finType}(l l':@language symbol):
+is_regular l/\is_regular l'->is_regular (l ∩ l').
+Proof.
+Close Scope language_scope.
+rewrite/is_regular=>[][][]state[]M H[]state'[]M' H'.
+exists (prod state state').
+exists (M × M')=>w.
+rewrite/cap_lang{}H{}H'/accept.
+suff H:(init (M × M') ・ dstar (delta (M × M')) w) ・ final (M × M') = 
+((init M ・ dstar (delta M) w) ・ final M )∩((init M' ・ dstar (delta M') w) ・ final M').
+rewrite{}H.
+split=>[[H H']|H].
+by rewrite H H' cap_idem.
+case:(@unit_empty_or_universal ((init M ・ dstar (delta M) w) ・ final M))=>H0;rewrite H0 in H *.
+rewrite cap_comm cap_empty in H.
+move:unit_identity_not_empty.
+by rewrite H.
+rewrite cap_comm cap_universal in H.
+by rewrite H unit_identity_is_universal.
 
+destruct M,M';simpl.
+move:init0 init1.
+elim:w=>[|h w H]init0 init1.
+by rewrite/=!comp_id_r sharpness/Rel_prod inv_cap_distr!comp_inv!(inv_invol (prod state state') _).
+move:(H(init0・delta0 h)(init1・delta1 h))=>{}H.
+rewrite/=-!comp_assoc-{}H.
+repeat f_equal.
+by rewrite{1 2}/Rel_prod!comp_assoc-sharpness-!comp_assoc/Rel_prod.
+
+Open Scope language_scope.
+Theorem regular_rev{symbol:finType}(l:@language symbol):
+is_regular l -> is_regular (l^r).
+Proof.
+Close Scope language_scope.
+rewrite/is_regular=>[][]state[]M H.
+exists state,(revM M)=>w.
+rewrite/rev_l{l}H/accept/revM/=.
+have H:forall (d:symbol->Rel state state)(w:seq symbol)(h:symbol),dstar d (rcons w h)=dstar d w・d h.
+move=>d{}w h.
+elim:w;[by rewrite/=comp_id_l comp_id_r|]=>a w H.
+by rewrite/=comp_assoc H.
+have{}H:dstar (fun x : symbol => delta M x #) w = dstar (delta M) (rev w) #.
+elim:w;[by rewrite inv_id|]=>h w H0.
+by rewrite/={}H0 rev_cons H comp_inv.
+by split=>H0;rewrite-inv_id-{}H0!comp_inv inv_invol comp_assoc H.
+Qed.
+
+
+Open Scope language_scope.
+Theorem regular_prod{symbol:finType}(l l':@language symbol):
+is_regular l /\ is_regular l' -> is_regular(l・l').
+Proof.
+Close Scope language_scope.
+rewrite/is_regular/accept/prod_lang=>[][][]state[]M H[]state'[]M' H'.
+exists (sum state state'),(concatM M M')=>w.
+remember (delta (concatM M M')) as d.
+remember (final (concatM M M')) as f.
+destruct M,M'.
+rewrite/= in H H' Heqd Heqf*.
+
+have{H'}H:(exists a b : seq symbol, w = a ++ b /\ l a /\ l' b)<->
+(exists a b : seq symbol, w = a ++ b /\
+(init0 ・ dstar delta0 a) ・ final0 = Id i /\
+(init1 ・ dstar delta1 b) ・ final1 = Id i).
+split=>[][]a[]b[]{}H0[]H1 H2;exists a,b;
+by[rewrite-H-H'|rewrite H H'].
+rewrite{l l'}H-Heqd-Heqf.
+
+have inil:forall init:Rel i state,init ・ Rel_sum (Id state) (init1 # ・ final0 #) #・inl_r state state'# = init.
+move=>init.
+by rewrite comp_assoc/Rel_sum comp_id_r inv_cup_distr!comp_inv
+2!inv_invol(inv_invol _ _(inr_r _ _))comp_cup_distr_r!comp_assoc
+inl_id inr_inl_empty!comp_empty_r cup_empty comp_id_r.
+
+have inir:forall init:Rel i state,init ・ Rel_sum (Id state) (init1 # ・ final0 #) #・inr_r state state'#= init・final0・init1.
+move=>init.
+by rewrite!comp_assoc/Rel_sum comp_id_r inv_cup_distr inv_invol!comp_inv
+inv_invol(inv_invol _ _(inr_r _ _))comp_cup_distr_r!comp_assoc
+inl_inr_empty inr_id cup_comm cup_empty comp_id_r.
+
+have rf:inr_r state state'・f = final1.
+rewrite Heqf-comp_assoc-{2}(@comp_id_l _ _ final1).
+f_equal.
+by rewrite/Rel_sum comp_cup_distr_l-!comp_assoc inr_inl_empty inr_id
+!comp_empty_l cup_comm comp_id_l cup_empty.
+
+have lf:inl_r state state'・f = final0・(init1・final1).
+rewrite Heqf-!comp_assoc.
+f_equal.
+by rewrite/Rel_sum comp_cup_distr_l-!comp_assoc inl_inr_empty inl_id
+comp_empty_l comp_id_l cup_empty.
+
+have {Heqf}inif:forall init:Rel i state,init ・ Rel_sum (Id state) (init1 # ・ final0 #) #・f = init・final0・(init1・final1).
+move=>init.
+rewrite Heqf!comp_assoc.
+f_equal.
+rewrite-!comp_assoc.
+f_equal.
+by rewrite sum_comp comp_inv 2!inv_invol inv_id comp_id_l comp_id_r cup_idem.
+
+have rdstar:forall w,inr_r state state'・dstar d w = dstar delta1 w・inr_r state state'.
+elim=>[|h{}w H].
+by rewrite/=comp_id_l comp_id_r.
+by rewrite/=-comp_assoc{1}Heqd/Rel_sum!comp_cup_distr_r!comp_cup_distr_l
+-!comp_assoc inr_id inr_inl_empty!comp_empty_l!comp_id_l cup_comm
+cup_empty cup_comm cup_empty!comp_assoc H.
+
+have rdstarf:forall w,inr_r state state'・(dstar d w・f) = dstar delta1 w・final1.
+move=>{}w.
+by rewrite-comp_assoc rdstar comp_assoc rf.
+
+have dstarl:forall w,dstar d w・inl_r state state'# =
+inl_r state state'#・dstar delta0 w.
+elim=>[|h{}w H].
+by rewrite/=comp_id_l comp_id_r.
+rewrite/=comp_assoc{}H-!comp_assoc.
+f_equal.
+by rewrite Heqd/Rel_sum!comp_cup_distr_r!comp_assoc inr_inl_empty inl_id
+comp_id_r comp_id_l!comp_empty_r!cup_empty.
+
+have inidstarl:forall (init:Rel i state)(w:seq symbol),init ・ Rel_sum (Id state) (init1 # ・ final0 #) #・dstar d w・inl_r state state'# =init・dstar delta0 w.
+move=>init{}w.
+by rewrite comp_assoc dstarl-comp_assoc inil.
+
+have{}Heqd:forall h,d h = inl_r state state'#・delta0 h・inl_r state state'∪
+(inl_r state state'#・final0・init1・delta1 h・inr_r state state')∪
+(inr_r state state'#・delta1 h・inr_r state state').
+move=>h.
+by rewrite Heqd/Rel_sum comp_id_r cup_assoc!comp_cup_distr_r!comp_assoc.
+
+split=>[[]a[]b[]H[]H0 H1|H].
+rewrite{w}H(_:dstar d(a++b)=dstar d a・dstar d b);[|
+by elim:{H0}a=>[|h a H];[rewrite/=comp_id_l|rewrite/=H comp_assoc]].
+
+rewrite-(comp_id_r _ _(dstar d a))-inl_inr_cup_id comp_cup_distr_l
+!comp_cup_distr_r comp_cup_distr_l comp_cup_distr_r-!comp_assoc inidstarl.
+suff:((((init0 ・ dstar delta0 a) ・ inl_r state state') ・ dstar d b) ・ f)=Id i.
+move=>H2.
+by rewrite H2 unit_identity_is_universal cup_comm cup_universal.
+
+move:H1.
+elim:b=>[|h b H].
+rewrite/=!comp_id_r=>H.
+by rewrite!comp_assoc lf H comp_id_r-comp_assoc H0.
+rewrite/=-!comp_assoc=>H1.
+
+by rewrite(comp_assoc i state)Heqd comp_cup_distr_l-!comp_assoc
+inl_inr_empty!comp_empty_l cup_empty!comp_assoc-comp_cup_distr_l
+comp_assoc-(comp_assoc state(sum _ _))inl_id comp_id_l
+!comp_cup_distr_r!comp_cup_distr_l!comp_assoc rdstarf-!comp_assoc
+H0 comp_id_l H1 unit_identity_is_universal cup_universal.
+
+move:init0 H.
+elim:w=>[|h w H]init0.
+rewrite/=comp_id_r inif.
+case:(@unit_empty_or_universal (init1 ・ final1))=>H.
+rewrite H!comp_empty_r=>{}H.
+move:unit_identity_not_empty.
+by rewrite H.
+rewrite H-unit_identity_is_universal comp_id_r=>H0.
+exists nil,nil.
+by rewrite/=!comp_id_r H H0 unit_identity_is_universal.
+
+rewrite/=Heqd!comp_cup_distr_r!comp_cup_distr_l comp_cup_distr_r
+-!comp_assoc inil inir comp_cup_distr_r!comp_assoc  rdstarf
+cup_assoc cup_idem.
+case:(@unit_empty_or_universal(init0 ・ (delta0 h ・ (inl_r state state' ・ (dstar d w ・ f)))))=>H1.
+rewrite H1 cup_comm cup_empty-comp_assoc=>{}H1.
+case:(@unit_empty_or_universal(init0 ・ final0))=>H2.
+rewrite H2 comp_empty_l in H1.
+move:unit_identity_not_empty.
+by rewrite H1.
+rewrite H2-unit_identity_is_universal comp_id_l in H1.
+exists nil,(h::w).
+by rewrite/=comp_id_r!comp_assoc H1 H2 unit_identity_is_universal.
+move=>_.
+have:((init0・ delta0 h ・ Rel_sum (Id state) (init1 # ・ final0 #) #) ・ dstar d w)・ f = Id i.
+by rewrite-(comp_id_l _ _(dstar d w))-inl_inr_cup_id!comp_assoc
+!comp_cup_distr_r!comp_cup_distr_l-!comp_assoc inil!comp_assoc H1
+cup_comm cup_universal unit_identity_is_universal.
+move/H=>[]a[]b[]{}H[]H0 H2.
+exists (h::a),b.
+by rewrite/=H-!comp_assoc H0 H2.
+Qed.
+
+Theorem regular_phi{symbol:finType}:@is_regular symbol phi.
+Proof.
+rewrite/is_regular.
+exists i,phiM=>w.
+by split;[|rewrite/accept/=!comp_empty_l=>H;move:unit_identity_not_empty;rewrite H].
+Qed.
+Theorem regular_eps{symbol:finType}:@is_regular symbol eps.
+rewrite/is_regular.
+exists i,epsM.
+rewrite/accept.
+case=>[|a l].
+by split=>[_|];[rewrite/=!comp_id_l|].
+rewrite/=comp_empty_l!comp_empty_r comp_empty_l.
+by split=>[|H];[|move:unit_identity_not_empty;rewrite H].
+Qed.
+
+Theorem regular_singl{symbol:finType}(s:symbol):is_regular(singl s).
+Proof.
+rewrite/is_regular.
+exists bool,(singlM s).
+rewrite/accept/inverse=>w.
+have H:forall a,a = Id i <-> a tt tt.
+move=>a.
+split=>H.
+by rewrite H.
+by case:( @unit_empty_or_universal a)=>H0;[rewrite H0 in H|rewrite H0 unit_identity_is_universal].
+
+rewrite H.
+case:w=>[|a[|b l]].
+split;[done|].
+by rewrite/=comp_id_r=>[][][[_]|[]].
+case_eq(s == a)=>/eqP{}H.
+subst.
+split=>[_|];[|done].
+exists false.
+split.
+exists true.
+by rewrite/=comp_id_r.
+done.
+(split;rewrite/singl)=>[[]H1|[]];[by subst|case=>[][]];[by simpl|].
+case=>[][[_]|[]].
+rewrite/=comp_id_r=>[][] _ [] H0.
+by subst.
+done.
+split.
+done.
+case=>[][][].
+by simpl.
+case=>[][[] _|[]];[|done].
+rewrite/==>[][][][][] _ [] H0.
+done.
+subst=>_.
+by case=>x[][].
+Qed.
+
+Open Scope language_scope.
+Theorem regular_comp{symbol:finType}(l:@language symbol):
+is_regular l -> is_regular (l^c).
+Proof.
+Close Scope language_scope.
+rewrite/is_regular/comp_lang=>[][]state[]M H.
+move:(NFA_DFA_equiv M)=>[]state'[]M'[]H0 H1.
+exists _,(compM M')=>w.
+rewrite{l}H{state M}H1.
+
+rewrite/accept/=.
+move:H0.
+rewrite/deterministic=>[][]H H0.
+have{H0}H:function_r(init M'・dstar(delta M')w).
+destruct M';rewrite/= in H H0 *.
+move:init0 H0.
+elim:w=>[|h w H1]init0 H0.
+by rewrite/=comp_id_r.
+rewrite/=-comp_assoc.
+apply/H1/function_comp/H/H0.
+have H0:exists x, (init M'・dstar(delta M')w)tt x.
+rewrite/function_r/total_r in H.
+move:H=>[]{}H _.
+have H0:Id i tt tt;[done|].
+move:(H tt tt H0)=>[]x[]{H0}H _.
+by exists x.
+case:H0=>x H0.
+have{}H:forall y,(init M' ・ dstar (delta M') w) tt y -> y=x.
+move=>y H1.
+rewrite/function_r/univalent_r in H.
+move:H=>[] _ H.
+have{H1}H0:((init M' ・ dstar (delta M') w) # ・ (init M' ・ dstar (delta M') w))x y.
+by exists tt.
+by move:(H _ _ H0).
+
+have{H0}H:forall R:Rel state' i,
+(init M' ・ dstar (delta M') w) ・ R = Id i <-> R x tt.
+move=>R.
+split=>H1.
+have:Id i tt tt;[done|rewrite-H1].
+case=>y[]/H{}H.
+by subst.
+by Rel_simpl=>[][][] _;[|exists x].
+by rewrite/not!H/complement/rpc.
+Qed.
+
+Theorem power_regular {symbol:finType}(l:@language symbol)(n:nat):
+is_regular l -> is_regular(power_l n l).
+Proof.
+move=>H.
+elim:n=>[|n H0].
+apply/regular_eps.
+by apply/regular_prod.
+Qed.
+
+Lemma dstar_cat {state symbol:finType}:
+forall(d:symbol->Rel state state)(a b:seq symbol),
+dstar d(a++b) = dstar d a・dstar d b.
+Proof.
+move=>d a b.
+elim:a=>[|h a H].
+by rewrite/=comp_id_l.
+by rewrite/=H comp_assoc.
+Qed.
+Lemma nil_rcons {symbol:Type}(s:seq symbol):s = nil \/exists t s',s=rcons s' t.
+Proof.
+elim:s=>[|h s[H|[]h'[]s']];[by left| |];right;
+[exists h,nil|exists h',(h::s')];by subst.
+Qed.
+Lemma dstar_rcons {state symbol:finType}:
+forall(d:symbol->Rel state state) w t,
+dstar d(rcons w t) = dstar d w・d t.
+Proof.
+move=>d w t.
+elim:w=>[|h w H].
+by rewrite/=comp_id_l comp_id_r.
+by rewrite/=H comp_assoc.
+Qed.
+
+
+Fixpoint take_reg {state symbol:finType}(init0:Rel i state)
+(delta0:symbol->Rel state state)(final0:Rel state i)(w:seq symbol)(n:nat):nat:=
+match n with
+|0 => size w
+|S n' =>
+  if is_true_inv(init0・dstar delta0(take n w)・final0 = Id i)
+  then n
+  else take_reg init0 delta0 final0 w n'
+end.
+
+Theorem plus_regular {symbol:finType}(l:@language symbol):
+is_regular l -> is_regular(plus_l l).
+Proof.
+rewrite/is_regular=>[][]state[]M H.
+exists _, (plus_nfa M)=>w.
+destruct M.
+rewrite/accept/plus_l/= in H *.
+
+remember(fun x : symbol =>
+delta0 x ∪ (delta0 x・(final0 ・ init0)))as d.
+
+split.
+case=>n.
+
+have H0:forall w, ((init0 ・ dstar delta0 w) ・ final0)
+⊆ ((init0 ・ dstar d w) ・ final0).
+move=>{}w.
+apply/comp_inc_compat_ab_a'b/comp_inc_compat_ab_ab'.
+elim:w=>[|h{}w{}H];[done|simpl=>x z[]y[]H0 H1].
+exists y.
+rewrite{1}Heqd.
+by split;[apply/cup_l|apply/H].
+
+move:w.
+elim:n=>[|n H1]w.
+rewrite/=/prod_lang=>[][]a[][|b' b[] _[] _];[|done].
+rewrite cats0=>[][]H1[]/H{}H _.
+subst.
+apply/inc_antisym_eq.
+by split;[rewrite unit_identity_is_universal|rewrite-{}H].
+
+rewrite/={1}/prod_lang=>[][]a[]b[]H2[]/H{}H/H1{}H1.
+rewrite{w}H2 dstar_cat.
+move:H.
+have H:(forall x:seq symbol,x = nil \/exists h x', x = rcons x' h).
+elim=>[|h x H];[by left|right].
+case:H=>H.
+exists h,nil.
+by subst.
+case:H=>x0[]x1 H.
+subst.
+by exists x0,(h::x1).
+case:(H a)=>[|[]t[]a']{}H.
+by rewrite{a}H/=comp_id_l.
+rewrite{a}H.
+have dstar_rcons:forall d,dstar d(rcons a' t) = dstar d a'・d t.
+move=>t0{Heqd H0 H1}d.
+elim:a'=>[|h a H].
+by rewrite/=comp_id_r comp_id_l.
+by rewrite/=H comp_assoc.
+rewrite!dstar_rcons=>H.
+rewrite{2}Heqd-!comp_assoc!comp_cup_distr_l!comp_cup_distr_r-!comp_assoc.
+have{}H:init0・dstar d a'・delta0 t・final0 = Id i.
+apply/inc_antisym_eq.
+split;[by rewrite unit_identity_is_universal|rewrite-{}H!comp_assoc].
+apply/comp_inc_compat_ab_ab'/comp_inc_compat_ab_a'b.
+elim:{dstar_rcons}a'=>[|h a H].
+done.
+rewrite/={1}Heqd comp_cup_distr_r comp_assoc-comp_cup_distr_l.
+apply/comp_inc_compat_ab_ab'=>x y/H.
+apply/cup_l.
+by rewrite H comp_id_l H1 unit_identity_is_universal cup_universal.
+
+move=>H0.
+have:exists u v, w = u ++ v /\ size v <= size w - 1 /\
+  init0・dstar delta0 u・final0・init0・dstar d v・final0 = Id i.
+have:Id i tt tt by [].
+rewrite-{1}H0=>[][]b[][]a[]{}H0 H1 H2.
+have:exists n, (take(S n)w = w/\(dstar delta0(take(S n)w)・final0) a tt) \/
+(dstar delta0(take(S n)w)・final0) a tt /\(init0・dstar d(drop(S n)w))tt b.
+move:a{H0}H1.
+elim:w=>[|h w H0]a.
+rewrite/=comp_id_l comp_id_r=>H1.
+have{}H1:a = b;[done|subst].
+exists 0.
+by left.
+rewrite/==>[][]c[]H1/H0[]n[][]{}H0 H3.
+rewrite Heqd in H1.
+case:H1=>alpha[][]H' H1;rewrite{alpha}H' in H1.
+exists (S n).
+rewrite H0 in H3 *.
+left.
+split;[done|].
+rewrite comp_assoc.
+by exists c.
+
+exists 0.
+right.
+rewrite take0 drop0/=comp_id_r.
+rewrite H0 in H3 *.
+rewrite-comp_assoc in H1.
+case:H1=>[][][]H1 H4.
+
+by rewrite/=comp_id_l comp_id_r.
+simpl.
+elim:w.
+rewrite/=!comp_id_r.
+remember a as a'.
+rewrite{}Heqa' in H1.
+move:a H1.
+elim:w=>[a H1|h w H1 a].
+have{}H1:a'=b;[done|subst].
+exists 0.
+rewrite/=comp_id_l comp_id_r.
+have H3:a' = b -> 
+
+have H3: final0 b tt /\ init0 tt b.
+move=>{}H.
+rewrite H/= in H1.
+by have{}H1:a = b;[|subst]. *)
+move:a{H0}H1 H2.
+
+elim:w=>[|h w H0]a H1 H2.
+rewrite/=comp_id_l in H1 *.
+exists 0.
+(* have:(nil:seq symbol)=nil;[done|]=>/H3{}H3. *)
+by have{}H1:a=b;[|subst].
+
+rewrite/= in H1 *.
+case:H1=>c[]H1 H'.
+(* have{}H3:(w = [::] -> final0 b tt /\ init0 tt b). *)
+(* move=>H4.
+rewrite H4/= in H'. *)
+
+(* apply/H3. *)
+move:(H0 _ H' H2)=>[]n[]{}H0.
+rewrite Heqd/cup/cupP in H1.
+case:H1=>alpha[][]H1 H4;rewrite{alpha}H1 in H4.
+exists (S n).
+rewrite comp_assoc.
+by split;[exists c|].
+exists 0.
+rewrite take0 drop0/=comp_id_r.
+rewrite-comp_assoc in H4.
+case:H4=>[][][]H1 H4.
+by split;[|exists c].
+
+case=>n[]H3 H4.
+exists (take(S n)w),(drop(S n)w).
+rewrite cat_take_drop.
+split;[done|].
+split.
+rewrite size_drop.
+case:(size w)=>[|n'];[done|].
+rewrite/=ssrnat.subSS PeanoNat.Nat.sub_0_r ssrnat.subnE.
+apply/PeanoNat.Nat.le_sub_l.
+remember(take(S n)w)as u.
+remember(drop(S n)w)as v.
+
+have H5:init0・dstar delta0 u・final0 = Id i.
+apply/inc_antisym_eq.
+split;[by rewrite unit_identity_is_universal|move=>[][] _].
+rewrite comp_assoc.
+by exists a.
+rewrite H5 comp_id_l.
+apply/inc_antisym_eq.
+split;[by rewrite unit_identity_is_universal|move=>[][] _].
+by exists b.
+case_eq(w == nil)=>/eqP H5.
+rewrite H5/=comp_id_r in H1 *.
+by have{}H1:a = b;[|subst;exists b].
+have{}H5:take(S n)w <> nil.
+case=>H6.
+have:size(take (S n) w)=0 by rewrite{}H6.
+rewrite size_take.
+case:(ssrnat.leq (S (S n)) (size w));[done|].
+move:{H1 H3 H4 H6}H5.
+by case:w.
+rewrite-(cat_take_drop(S n)w)dstar_cat in H1.
+case:H1=>c[]H1{}H4.
+exists b.
+split;[|done].
+exists c.
+split;[|done].
+have{}H1:dstar d()
+have H5:take (S n) w = nil -> init0 tt c.
+move=>H5.
+rewrite H5/= in H1.
+by have{}H1:a = c;[|subst].
+move:a H1 H3 H5{H0}.
+elim:(take(S n)w)=>[|h t H1]a.
+move=>_ _ H1.
+by have:(nil:seq symbol) = nil=>[|/H1].
+rewrite/==>[][]e[]H3/H1{}H1.
+
+rewrite/==>_{}H1.
+have{}H1:a = c by [].
+by subst.
+rewrite/=.
+case:H1=>t[]s H1.
+rewrite H1!dstar_rcons{2}Heqd comp_cup_distr_l.
+
+elim:(take(S n)w)=>[|a0 l0 H1].
+rewrite/==>_ H1.
+
+
+move=>[][] _.
+Search ( _ - _ <= _).
+done.
+case:w.
+case_eq(take(S n)w)=>H4.
+have:size(take(S n)w)=0 by rewrite H4.
+rewrite size_take.
+
+rewrite/not.
+remember (take(S n)w) as u.
+have{H0 H1 H2}
+
+case:H2=>d[]H1[][][]H2 H5.
+exists (S n),e.
+split.
+
+
+done.
+H3 H4.
+subst.
+
+
+rewrite/={1}Heqd/cup/cupP=>[][]c[][]alpha[][]H1 H2 H3;[left|right].
+
+
+rewrite/={1}Heqd/cup/cupP=>H1[]c[][]alpha[][]H2 H3 H4 H5.
+admit.
+subst.
+case:H3=>d[]H3[][][]H6 H7.
+move:(H0 a b H1).
+move:(H0 c b )
+exists (S n),c.
+rewrite H2.
+rewrite Heqd
+
+have H1:exists n, init0・dstar delta0(take(S n)w)・final0 = Id i.
+
+(* have:size w < S(size w) by [].
+remember(S(size w))as n=>{Heqn}.
+move:w.
+elim:n=>[|n H0]w.
+by move/PeanoNat.Nat.nlt_0_r.
+move=>H1 H2. *)
+exists (take_reg init0 delta0 final0 w (size w)).
+
+
+move=>H0.
+have H1:exists n, init0・dstar d(take n w)・final0 = Id i.
+move:H0.
+elim:w=>[|h w{}H].
+rewrite/=comp_id_r=>{}H.
+by exists 0.
+
+have{}H0:exists n,
+init0・dstar d(take(S n)w)・final0・init0・dstar delta0(drop(S n)w)・final0 = Id i.
+case:(Classical_Prop.classic (exists n : nat,
+((((init0 ・ dstar d (take (S n) w)) ・ final0) ・ init0)
+・ dstar delta0 (drop (S n) w)) ・ final0 = Id i)).
+done.
+move/Classical_Pred_Type.not_ex_all_not=>H1.
+exfalso.
+have [n]: exists n : nat, True by exists 0.
+move:(H1 n)=>{}H1.
+exfalso.
+move:H1.
+elim:n.
+
+fix_rcons
+Search (~ (_ /\ _)).
+move=> (n0 : nat).
+pose n:nat.
+move=>n.
+move=>n.
+elim:H1.
+Search (~ (exists _, _)). 
+move:H0.
+elim:w=>[|h w H0].
+rewrite H/=.
+by left.
+rewrite/=comp_assoc{1}Heqd!comp_cup_distr_r comp_cup_distr_l-!comp_assoc=>H1.
+case:( @unit_empty_or_universal (init0・delta0 h・dstar d w・final0))=>H2.
+rewrite{}H2 cup_comm cup_empty in H1.
+right.
+case:( @unit_empty_or_universal((init0 ・ delta0 h) ・ final0))=>H2.
+rewrite H2!comp_empty_l in H1.
+move:unit_identity_not_empty.
+by rewrite H1.
+rewrite-unit_identity_is_universal in H2.
+rewrite H2 comp_id_l in H1.
+exists [::h],w.
+by rewrite/=comp_id_r H2 H1.
+left.
+rewrite H/=unit_identity_is_universal-!comp_assoc .
+
+
+
+
+
+
+
+case:(Classical_Prop.classic(exists n : nat, prod_lang l (power_l n l) w)).
+done.
+rewrite/not=>H0 H1.
+exfalso.
+case:H0.
+exfalso.
+apply/contrapositive.
+
+
+case:w=>[|h w].
+rewrite/=/prod_lang=>H0.
+exists 0,nil,nil.
+by rewrite H/=.
+
+
+
+rewrite/={1}Heqd!comp_cup_distr_r comp_cup_distr_l comp_cup_distr_r
+comp_id_l-!comp_assoc=>H0.
+have{}H0:(((init0 ・ delta0 h) ・ dstar d w) ・ final0) = Id i.
+case:( @unit_empty_or_universal (init0・final0))=>H1.
+by rewrite H1!comp_empty_l cup_empty in H0.
+by rewrite H1-unit_identity_is_universal comp_id_l cup_idem in H0.
+
+
+
+
+have H0:forall w,plus_l l w -> l w \/ (exists u v, w = u ++ v/\l u /\ plus_l l v).
+move=>{}w[]n.
+move:n w.
+elim=>[|n];[left|].
+by case:p=>a[][[]H0[]H1 _|b' b[] _ [] _];[rewrite H0 cats0|].
+
+remember (S n) as n'=>H0 w.
+rewrite/==>[][]a[]b[]H1[]H2/H0[];right.
+exists a,b.
+split;[done|split;[done|]].
+exists 0,b,nil.
+by rewrite cats0.
+exists a,b.
+split;[done|split;[done|]].
+rewrite/plus_l.
+exists 0.
+case=>x[]y[].
+rewrite/power_l
+
+
+done.
+case=>[][[]a[][[]H0[]H1 _|b' b[] _ [] _]|n].
+rewrite cats0 in H0.
+left.
+by subst.
+done.
+rewrite/=
+case=>a[]b.
+
+
+
+case:w=>[|h w].
+rewrite/=/prod_lang=>H0.
+exists 0,nil,nil.
+by rewrite H/=.
+
+rewrite/={1}Heqd!comp_cup_distr_r!comp_cup_distr_l!comp_cup_distr_r
+comp_id_l-!comp_assoc=>H0.
+have{}H0:(((init0 ・ delta0 h) ・ dstar d w) ・ final0) = Id i.
+case:( @unit_empty_or_universal (init0 ・ final0))=>H1;rewrite H1 in H0.
+by rewrite!comp_empty_l cup_empty in H0.
+by rewrite-unit_identity_is_universal comp_id_l cup_idem in H0.
+rewrite/prod_lang.
+exists 0.
+split;[done|split=>[|]].
+rewrite/=.
+
+
+
+rewrite/=!comp_cup_distr_r!comp_cup_distr_l!comp_cup_distr_r!comp_id_l=>H2.
+
+Search (_ ⊆ (_ ∪ _)).
+rewrite/==>H.
+Search ((_ ・_)⊆(_・_)).
+apply/
+
+admit.
+
+elim:w=>[|h w H0].
+rewrite/=comp_id_r/prod_lang=>H0.
+exists 0,nil,nil.
+by rewrite H/=comp_id_r.
+rewrite/=-comp_assoc.
+
+
+rewrite/=comp_id_r/prod_lang.
+split=>[|H0].
+case=>n[][|a' a][][|b' b][];[|done|done|done].
+by rewrite H/=comp_id_r=>[] _[]{}H.
+exists 0,nil,nil.
+by rewrite H/=comp_id_r.
+
+split.
+
+move:H.
+simpl.
+simpl.
+
+simpl.
+done.
+done.
+done.
+
+
+
+split.
+case=>x.
+rewrite/prod_lang.
+elim:x=>[|n H0].
+rewrite/=/prod_lang/eps=>[][]a[]b[]H0[]/H{}H H1.
+rewrite{b}H1 cats0 in H0.
+subst.
+
+apply/inc_antisym;[by rewrite unit_identity_is_universal|rewrite-{}H].
+apply/comp_inc_compat_ab_a'b/comp_inc_compat_ab_ab'.
+elim:a=>[|h w H];[done|].
+rewrite/=comp_cup_distr_r comp_id_l.
+apply/(inc_trans state state(delta0 h・dstar delta0 w)
+(delta0 h・dstar (fun x : symbol => (Id state ∪ (final0 ・ init0)) ・ delta0 x)w )
+((delta0 h ∪ ((final0 ・ init0) ・ delta0 h))
+・ dstar (fun x : symbol => (Id state ∪ (final0 ・ init0))
+・ delta0 x) w))/comp_inc_compat_ab_a'b/cup_l/comp_inc_compat_ab_ab'/H.
+
+rewrite/=.
+
+remember (S n) as n'=>{n Heqn'}
+.
+
+
+simpl.
+
+
+
+Search (_⊆(_∪_)).
+apply/inc_comp_r.
+
+Rel_simpl.
+by rewrite unit_identity_is_universal.
+case:H=>H _.
+apply (inc_trans i i ((init0 ・ dstar delta0 a) ・ final0)(Id i)
+((init0
+・ dstar (fun x : symbol => (Id state ∪ (final0 ・ init0))
+・ delta0 x) a) ・ final0) H).
+apply/H.
+simpl.
+
+
+admit.
+move.
